update

Playground/Misc/Logic.lean
@@ -1,11 +1,17 @@
 import Std.Data.List.Lemmas
 import Playground.Data.Fin.Family.Basic
+import Playground.Data.Fin.Family.Sum
 namespace Logic
 
 section
   structure FOL where
     function : Nat → Type
     relation : Nat → Type
+    fdeq : ∀ n, DecidableEq (function n)
+    rdeq : ∀ n, DecidableEq (relation n)
+
+  instance (language : FOL) (n) : DecidableEq (language.function n) := language.fdeq n
+  instance (language : FOL) (n) : DecidableEq (language.relation n) := language.rdeq n
   
   abbrev Var := Nat
   abbrev PropVar := Nat
@@ -25,14 +31,16 @@ section
   | app : (n : Nat) → language.relation n → (Fin n → Term language) → Formula
   | all : Var → Formula → Formula
   | ex : Var → Formula → Formula
+  | eq : Term language → Term language → Formula
 
   scoped infixr:35 " ∧ "   => Formula.and
   scoped infixr:30 " ∨  "  => Formula.or
   scoped infixr:2 " ⇒ "   => Formula.imp
   scoped notation:max "⊥" => Formula.bot
   scoped notation:max "¬" p => (p ⇒ ⊥)
-  scoped notation:max "∀ " x ";" f => Formula.all x f
-  scoped notation:max "∃ " x ";" f => Formula.ex x f
+  scoped notation:max "∀ " x "; " f => Formula.all x f
+  scoped notation:max "∃ " x "; " f => Formula.ex x f
+  scoped infixr:50 " ≡ " => Formula.eq
 
   section
     variable {language : FOL}
@@ -61,14 +69,70 @@ section
     def decidable_Mem (v : Var) : (t : Term language) → Decidable (v ∈ t)
       | .var x => by
         rw [Mem_var_iff]
-        exact inferInstance
+        infer_instance
       | .app n f l => by
         rw [Mem_app_iff]
         let r k := decidable_Mem v (l k)
-        exact inferInstance
+        infer_instance
 
     instance (v : Var) : (t : Term language) → Decidable (v ∈ t) := decidable_Mem v
+
     end Term.Mem
+
+    def Term.decidable_Eq : DecidableEq (Term language)
+    | var .., app ..
+    | app .., var .. => isFalse Term.noConfusion
+    | var .., var .. => by rw [var.injEq]; infer_instance
+    | app n f l, app n' f' l' => by
+      rw [app.injEq]
+      exact if hn : n = n' then by
+        subst hn
+        let _ := λ k => decidable_Eq (l k) (l' k)
+        simp; infer_instance
+      else isFalse λ c => hn c.1
+
+    instance : DecidableEq (Term language) := Term.decidable_Eq
+
+    def Formula.decidable_Eq : DecidableEq (Formula language)
+    | propVar .., propVar .. => by rw [propVar.injEq]; infer_instance
+    | and .., or .. | and .., imp .. | and .., bot .. | and .., propVar .. 
+    | and .., app .. | and .., all .. | and .., ex .. | and .., eq .. => isFalse Formula.noConfusion
+    | or .., and .. | or .., imp .. | or .., bot .. | or .., propVar .. 
+    | or .., app .. | or .., all .. | or .., ex .. | or .., eq .. => isFalse Formula.noConfusion
+    | imp .., and .. | imp .., or .. | imp .., bot .. | imp .., propVar .. 
+    | imp .., app .. | imp .., all .. | imp .., ex .. | imp .., eq .. => isFalse Formula.noConfusion
+    | bot .., and .. | bot .., or .. | bot .., imp .. | bot .., propVar .. 
+    | bot .., app .. | bot .., all .. | bot .., ex .. | bot .., eq .. => isFalse Formula.noConfusion
+    | propVar .., and .. | propVar .., or .. | propVar .., imp .. | propVar .., bot ..
+    | propVar .., app .. | propVar .., all .. | propVar .., ex .. | propVar .., eq .. => isFalse Formula.noConfusion
+    | app .., and .. | app .., or .. | app .., imp .. | app .., bot .. | app .., propVar .. 
+    | app .., all .. | app .., ex .. | app .., eq .. => isFalse Formula.noConfusion
+    | all .., and .. | all .., or .. | all .., imp .. | all .., bot .. | all .., propVar .. 
+    | all .., app .. | all .., ex .. | all .., eq .. => isFalse Formula.noConfusion
+    | ex .., and .. | ex .., or .. | ex .., imp .. | ex .., bot .. | ex .., propVar .. 
+    | ex .., app .. | ex .., all .. | ex .., eq .. => isFalse Formula.noConfusion
+    | eq .., and .. | eq .., or .. | eq .., imp .. | eq .., bot .. | eq .., propVar .. 
+    | eq .., app .. | eq .., all .. | eq .., ex .. => isFalse Formula.noConfusion
+    | and f g, and f' g' => by
+      rw [and.injEq]; let _ := decidable_Eq f f'; let _ := decidable_Eq g g'
+      infer_instance
+    | or f g, or f' g' => by
+      rw [or.injEq]; let _ := decidable_Eq f f'; let _ := decidable_Eq g g'
+      infer_instance
+    | imp f g, imp f' g' => by
+      rw [imp.injEq]; let _ := decidable_Eq f f'; let _ := decidable_Eq g g'
+      infer_instance
+    | bot, bot => isTrue rfl
+    | all x f, all x' f' => by rw [all.injEq]; let _ := decidable_Eq f f'; infer_instance
+    | ex x f, ex x' f' => by rw [ex.injEq]; let _ := decidable_Eq f f'; infer_instance
+    | eq a b, eq a' b' => by rw [eq.injEq]; infer_instance
+    | app n f l, app n' f' l' => by
+      rw [app.injEq]
+      exact if hn : n = n' then by subst hn; simp; infer_instance
+      else isFalse λ c => hn c.1
+
+    instance : DecidableEq (Formula language) := Formula.decidable_Eq
+
 
     inductive Formula.Mem (v : Var) : Formula language → Prop
     | and_l {f g : Formula _} : f.Mem v → (f ∧ g).Mem v
@@ -82,6 +146,8 @@ section
     | all_x {f} : (∀ v; f).Mem v
     | ex_f {x} {f} : f.Mem v → (∃ x; f).Mem v
     | ex_x {f} : (∃ v; f).Mem v
+    | eq_l {a b : Term _} : a.Mem v → (a ≡ b).Mem v
+    | eq_r {a b : Term _} : b.Mem v → (a ≡ b).Mem v
 
     instance : Membership Var (Formula language) where mem := Formula.Mem
 
@@ -92,7 +158,8 @@ section
       let motive : (t : Formula language) → v ∈ t → Prop := 
         λ | .and f' g', _ => (v ∈ f' ∨ v ∈ g') | _, _ => True
       rec (motive := motive) (and_l := λ h _ => Or.inl h) (and_r := λ h _ => Or.inr h)
-        (by simp) (by simp) (by simp) (by simp) (by simp) (by simp) (by simp) (by simp) (by simp)
+        (by simp) (by simp) (by simp) (by simp) (by simp) (by simp) 
+        (by simp) (by simp) (by simp) (by simp) (by simp)
       , λ | .inl h => .and_l h | .inr h => .and_r h⟩
 
     theorem Mem_or_iff (v : Var) (f g : Formula language)
@@ -100,7 +167,8 @@ section
       let motive : (t : Formula language) → v ∈ t → Prop := 
         λ | .or f' g', _ => (v ∈ f' ∨ v ∈ g') | _, _ => True
       rec (motive := motive) (or_l := λ h _ => Or.inl h) (or_r := λ h _ => Or.inr h)
-        (by simp) (by simp) (by simp) (by simp) (by simp) (by simp) (by simp) (by simp) (by simp)
+        (by simp) (by simp) (by simp) (by simp) (by simp) (by simp) 
+        (by simp) (by simp) (by simp) (by simp) (by simp)
       , λ | .inl h => .or_l h | .inr h => .or_r h⟩
 
     theorem Mem_imp_iff (v : Var) (f g : Formula language)
@@ -108,7 +176,8 @@ section
       let motive : (t : Formula language) → v ∈ t → Prop := 
         λ | .imp f' g', _ => (v ∈ f' ∨ v ∈ g') | _, _ => True
       rec (motive := motive) (imp_l := λ h _ => Or.inl h) (imp_r := λ h _ => Or.inr h)
-        (by simp) (by simp) (by simp) (by simp) (by simp) (by simp) (by simp) (by simp) (by simp)
+        (by simp) (by simp) (by simp) (by simp) (by simp) (by simp) 
+        (by simp) (by simp) (by simp) (by simp) (by simp)
       , λ | .inl h => .imp_l h | .inr h => .imp_r h⟩
 
     theorem Mem_bot_iff (v : Var)
@@ -116,7 +185,8 @@ section
       let motive : (t : Formula language) → v ∈ t → Prop := 
         λ | .bot, _ => False | _, _ => True
       rec (motive := motive) (by simp) (by simp)
-        (by simp) (by simp) (by simp) (by simp) (by simp) (by simp) (by simp) (by simp) (by simp)
+        (by simp) (by simp) (by simp) (by simp) (by simp) (by simp) 
+        (by simp) (by simp) (by simp) (by simp) (by simp)
       , False.elim⟩
 
     theorem Mem_propVar_iff (v : Var) {x}
@@ -124,7 +194,8 @@ section
       let motive : (t : Formula language) → v ∈ t → Prop := 
         λ | .propVar _, _ => False | _, _ => True
       rec (motive := motive) (by simp) (by simp)
-        (by simp) (by simp) (by simp) (by simp) (by simp) (by simp) (by simp) (by simp) (by simp)
+        (by simp) (by simp) (by simp) (by simp) (by simp) (by simp) 
+        (by simp) (by simp) (by simp) (by simp) (by simp)
       , False.elim⟩
 
     theorem Mem_app_iff (v : Var) (n) (f) (l) 
@@ -132,7 +203,8 @@ section
       let motive : (t : Formula language) → v ∈ t → Prop := 
         λ | .app _ _ l', _ => (∃ k, v ∈ l' k) | _, _ => True
       rec (motive := motive) (app := λ h => ⟨_, h⟩) (by simp)
-        (by simp) (by simp) (by simp) (by simp) (by simp) (by simp) (by simp) (by simp) (by simp)
+        (by simp) (by simp) (by simp) (by simp) (by simp) (by simp) 
+        (by simp) (by simp) (by simp) (by simp) (by simp)
       , λ ⟨_, h⟩ => .app h⟩
 
     theorem Mem_all_iff (v : Var) (x) (f : Formula language)
@@ -140,7 +212,8 @@ section
       let motive : (t : Formula language) → v ∈ t → Prop := 
         λ | .all x' f', _ => (v = x' ∨ v ∈ f') | _, _ => True
       rec (motive := motive) (all_x := Or.inl rfl) (all_f := λ h _ => Or.inr h)
-        (by simp) (by simp) (by simp) (by simp) (by simp) (by simp) (by simp) (by simp) (by simp)
+        (by simp) (by simp) (by simp) (by simp) (by simp) (by simp) 
+        (by simp) (by simp) (by simp) (by simp) (by simp)
       , λ | .inl h => h ▸ .all_x | .inr h => .all_f h⟩
 
     theorem Mem_ex_iff (v : Var) (x) (f : Formula language)
@@ -148,67 +221,73 @@ section
       let motive : (t : Formula language) → v ∈ t → Prop := 
         λ | .ex x' f', _ => (v = x' ∨ v ∈ f') | _, _ => True
       rec (motive := motive) (ex_x := Or.inl rfl) (ex_f := λ h _ => Or.inr h)
-        (by simp) (by simp) (by simp) (by simp) (by simp) (by simp) (by simp) (by simp) (by simp)
+        (by simp) (by simp) (by simp) (by simp) (by simp) (by simp) 
+        (by simp) (by simp) (by simp) (by simp) (by simp)
       , λ | .inl h => h ▸ .ex_x | .inr h => .ex_f h⟩
+
+    theorem Mem_eq_iff (v : Var) (a b : Term language)
+      : v ∈ (a ≡ b) ↔ (v ∈ a ∨ v ∈ b) := ⟨
+      let motive : (t : Formula language) → v ∈ t → Prop := 
+        λ | .eq a' b', _ => (v ∈ a' ∨ v ∈ b') | _, _ => True
+      rec (motive := motive) (eq_l := λ h => Or.inl h) (eq_r := λ h => Or.inr h)
+        (by simp) (by simp) (by simp) (by simp) (by simp) (by simp) 
+        (by simp) (by simp) (by simp) (by simp) (by simp)
+      , λ | .inl h => .eq_l h | .inr h => .eq_r h⟩
 
     def decidable_Mem (v : Var) : (t : Formula language) → Decidable (v ∈ t)
       | .and f g => by
         rw [Mem_and_iff]
         let _ := decidable_Mem v f; let _ := decidable_Mem v g
-        exact inferInstance
+        infer_instance
       | .or f g => by
         rw [Mem_or_iff]
         let _ := decidable_Mem v f; let _ := decidable_Mem v g
-        exact inferInstance
+        infer_instance
       | .imp f g => by
         rw [Mem_imp_iff]
         let _ := decidable_Mem v f; let _ := decidable_Mem v g
-        exact inferInstance
+        infer_instance
       | .bot => by
         rw [Mem_bot_iff]
-        exact inferInstance
+        infer_instance
       | .propVar x => by
         rw [Mem_propVar_iff]
-        exact inferInstance
+        infer_instance
       | .app n f l => by
         rw [Mem_app_iff]
-        exact inferInstance
+        infer_instance
       | .all x f => by
         rw [Mem_all_iff]
         let _ := decidable_Mem v f
-        exact inferInstance
+        infer_instance
       | .ex x f => by
         rw [Mem_ex_iff]
         let _ := decidable_Mem v f
-        exact inferInstance
+        infer_instance
+      | .eq a b => by
+        rw [Mem_eq_iff]
+        infer_instance
 
     instance (v : Var) : (f : Formula language) → Decidable (v ∈ f) := decidable_Mem v 
 
     end Formula.Mem
 
-    -- instance : Membership Var (List (Term language)) where
-    --   mem v l := ∃ t ∈ l, v ∈ t
-    -- instance : Membership Var (List (Formula language)) where
-    --   mem v l := ∃ t ∈ l, v ∈ t
-    -- instance : Membership Var (List (Formula language ⊕ Term language)) where
-    --   mem v l := ∃ t ∈ l, match t with | .inl t => v ∈ t | .inr t => v ∈ t
-
-
     def Term.subst (v : Var) (t : Term language) : Term language → Term language
     | var x => if x = v then t else var x
     | app n f l => app n f (λ i => subst v t (l i))
-    scoped notation:40 u "[" v ":=" t "]"  => Term.subst v t u
+    scoped notation:max u "[" v ":=" t "]"  => Term.subst v t u
 
     inductive Formula.ValidSubst (v : Var) (t : Term language) : Formula language → Type
     | and {f g : Formula _} : f.ValidSubst v t → g.ValidSubst v t → (f ∧ g).ValidSubst v t
     | or {f g : Formula _} : f.ValidSubst v t → g.ValidSubst v t → (f ∨ g).ValidSubst v t
     | imp {f g : Formula _} : f.ValidSubst v t → g.ValidSubst v t → (f ⇒ g).ValidSubst v t
-    | bot : ⊥.ValidSubst v t
+    | bot : (⊥ : Formula _).ValidSubst v t
     | propVar : (propVar ..).ValidSubst v t
     | app : (app ..).ValidSubst v t
     | all {x} {f} : v ≠ x → x ∉ t → f.ValidSubst v t → (∀ x; f).ValidSubst v t
     | ex {x} {f} : v ≠ x → x ∉ t → f.ValidSubst v t → (∃ x; f).ValidSubst v t
-    scoped notation:40 p "[" v ":=" t "] valid" => Formula.ValidSubst v t p
+    | eq {a b : Term language} : (a ≡ b).ValidSubst v t
+    scoped notation:max p "[" v ":=" t "] valid" => Formula.ValidSubst v t p
 
     def Formula.subst (v : Var) (t : Term language)
       : (f : Formula language) → f[v := t] valid → Formula language
@@ -220,10 +299,11 @@ section
     | app n f l, _ => app n f (λ k => (l k)[v := t])
     | all x p, .all _ _ h3 => all x (p.subst v t h3)
     | ex x p, .ex _ _ h3 => ex x (p.subst v t h3)
-    scoped notation:40 p "[" v ":=" t "," h "]"  => Formula.subst v t p h
+    | eq a b, _ => eq a[v := t] b[v := t]
+    scoped notation:max p "[" v ":=" t "," h "]"  => Formula.subst v t p h
 
     open Formula in
-    inductive Proof : List (Formula language) → Formula language → Prop
+    inductive Proof : List (Formula language) → Formula language → Type
     | ax : p ∈ s → Proof s p
     | weaken (t) : Proof s p → Proof (t :: s) p
     | and_intro : Proof s p → Proof s q → Proof s (p ∧ q)
@@ -236,34 +316,63 @@ section
     | imp_elim : Proof s p → Proof s (p ⇒ q) → Proof s q
     | bot_elim (p) : Proof s ⊥ → Proof s p
     | lem (p) : Proof s (p ∨ ¬p)
-    | all_intro {s} (x) (hsx : ∀ f, f ∈ s → x ∉ f) : Proof s p → Proof s (∀ x; p)
-    | all_elim (ht : p[x := t] valid) : Proof s (∀ x; p) → Proof s (p[x := t, ht])
-    | ex_intro {ht : p[x := t] valid} : Proof s (p[x := t, ht]) → Proof s (∃ x; p)
-    | ex_elim {s} (hsx : ∀ f, f ∈ s → x ∉ f) (hqx : x ∉ q) : Proof s (∃ x; p) → Proof (p :: s) q → Proof s q
+    | all_intro (x) (hsx : ∀ f, f ∈ s → x ∉ f) : Proof s p → Proof s (∀ x; p)
+    | all_elim (ht : p[x := t] valid) : Proof s (∀ x; p) → Proof s p[x := t, ht]
+    | ex_intro {ht : p[x := t] valid} : Proof s p[x := t, ht] → Proof s (∃ x; p)
+    | ex_elim (hsx : ∀ f, f ∈ s → x ∉ f) (hqx : x ∉ q) : Proof s (∃ x; p) → Proof (p :: s) q → Proof s q
+    | eq_intro (t) : Proof s (t ≡ t)
+    | eq_elim (t) (ht : p[x := t] valid) (hu : p[x := u] valid)
+      :  Proof s (t ≡ u) → Proof s p[x := t, ht] → Proof s p[x := u, hu]
 
-    scoped infix:1 " ⊢ " => Proof
-    scoped notation:1 "⊢ " f => Proof ∅ f
-    scoped notation:1 s " ⊢[" L "] " f => Proof (language := L) s f
-    scoped notation:1 "⊢[" L "] " f => Proof (language := L) ∅ f
+
+    scoped notation:max s " ⊢ " f => (Proof s f)
+    scoped notation:max "⊢ " f => (Proof ∅ f)
+    scoped notation:max s " ⊢[" L "] " f => (Proof (language := L) s f)
+    scoped notation:max "⊢[" L "] " f => (Proof (language := L) ∅ f)
 
 
     def Term.newFreshVar : Term language → Var
-    | var x => (x : Nat).succ
-    | app n f l => 
-      sorry
+    | var x => (x : Nat) + 1
+    | app n f l => (Fin.Family.of λ k => (l k).newFreshVar).sum 0 + 1
 
-    theorem Term.all_vars_lt_newFreshVar
+    theorem Term.lt_newFreshVar_of_Mem
       : ∀ (t : Term language), ∀ ⦃v⦄, v ∈ t → v < t.newFreshVar
     | var x, v, hv => 
-      -- (x : Nat).lt_succ_self
-      sorry
-    | _, _, _ => sorry
+      have hv := (Term.Mem.Mem_var_iff ..).mp hv
+      hv ▸ by simp_arith [newFreshVar]
+    | app n f l, v, hv => 
+      have ⟨k, h⟩ := (Term.Mem.Mem_app_iff ..).mp hv
+      have h := lt_newFreshVar_of_Mem _ h
+      have := (Fin.Family.of λ k => (l k).newFreshVar).sum_ge k
+      Nat.lt_trans h (Nat.lt_succ_of_le this)
 
-    theorem Term.newFreshVar_not_in : ∀ (t : Term language), t.newFreshVar ∉ t :=
-      sorry
+    theorem Term.newFreshVar_not_Mem (t : Term language) : t.newFreshVar ∉ t :=
+      λ c => Nat.lt_irrefl _ (t.lt_newFreshVar_of_Mem c)
+    
+    theorem Term.subst_of_not_Mem {x} {t : Term language} (u : Term language) (h : x ∉ t)
+      : t[x := u] = t :=
+        match t with
+        | var v => by
+          show ite .. = _
+          rw [Mem.Mem_var_iff] at h
+          rw [if_neg λ c => h c.symm]
+        | app n f l => by
+          show app .. = app ..
+          rw [Mem.Mem_app_iff] at h
+          apply congr_arg
+          funext i
+          exact (l i).subst_of_not_Mem u λ c => h ⟨i, c⟩
+
+    def Proof.eq_symm {s} {t u : Term language} (h : s ⊢ t ≡ u) : s ⊢ u ≡ t :=
+      let x := t.newFreshVar
+      have hx := t.newFreshVar_not_Mem
+      let p := .var x ≡ t
+      let vz : ∀ z, p[x := z] valid := λ z => by apply Formula.ValidSubst.eq
+      have sz : ∀ z, p[x := z, vz z] = (z ≡ t) := λ z =>
+        by dsimp [Formula.subst]; rw [Term.subst_of_not_Mem z hx]; simp [Term.subst]
+      sz u ▸ eq_elim t (vz t) (vz u) h <| sz t ▸ eq_intro t
 
   end
-
 
   section
     open Formula Proof
@@ -279,6 +388,148 @@ section
             <| imp_elim (ax <| by simp)
               <| weaken _ h
     def of_notnot : (s ⊢ ¬¬p) → (s ⊢ p) := absurd_r
+  end
+
+  section
+  -- semantics
+  structure Interpretation (language : FOL) where
+    propValue (p : Nat) : Bool
+    domain : Type
+    varValue (x : Nat) : domain
+    functionValue (n : Nat) (f : language.function n) : (Fin n → domain) → domain
+    relationValue (n : Nat) (r : language.relation n) : (Fin n → domain) → Bool
+
+  def Term.value {language} (i : Interpretation language) : Term language → i.domain
+  | var x => i.varValue x
+  | app _ f l => i.functionValue _ f λ k => (l k).value i
+
+  scoped notation:max "⟦" t " | " i "⟧"  => (Term.value i t)
+
+  def Interpretation.setPropValue {language} (i : Interpretation language) (v : Nat) (d : Bool) 
+  : Interpretation language := 
+  { i with propValue := λ a => if a = v then d else i.propValue a }
+
+  def Interpretation.setVarValue {language} (i : Interpretation language) (v : Nat) (d : i.domain) 
+  : Interpretation language := 
+  { i with varValue := λ a => if a = v then d else i.varValue a }
+
+  scoped notation:max i "⟦" v ":=" d "⟧" => (Interpretation.setVarValue i v d)
+
+  -- todo: change this to inductive
+  def Formula.isTrueUnder {language} (i : Interpretation language) : Formula language → Prop
+  | and f g => f.isTrueUnder i ∧ g.isTrueUnder i
+  | or f g => f.isTrueUnder i ∨ g.isTrueUnder i
+  | imp f g => f.isTrueUnder i → g.isTrueUnder i
+  | bot => False
+  | propVar x => i.propValue x = true
+  | app _ f l => (i.relationValue _ f λ k => ⟦l k | i⟧) = true
+  | all x f => ∀ d, f.isTrueUnder i⟦x := d⟧
+  | ex x f => ∃ d, f.isTrueUnder i⟦x := d⟧
+  | eq a b => ⟦a | i⟧ = ⟦b | i⟧
+
+  scoped notation:max "⊨[" i "] " f  => (Formula.isTrueUnder i f)
+  def Formula.isTrue {language} (f : Formula language) := ∀ i, ⊨[i] f
+  scoped notation:max "⊨ " f  => (Formula.isTrue f)
+  def Formula.entailsUnder {language} (i : Interpretation language) 
+    (s : List (Formula language)) (f : Formula language) := (∀ x ∈ s, ⊨[i] x) → ⊨[i] f
+  scoped notation:max s " ⊨[" i "] " f  => (Formula.entailsUnder i s f)
+  def Formula.entails {language} (s : List (Formula language)) (f : Formula language) := ∀ i, s ⊨[i] f
+  scoped notation:max s " ⊨ " f  => (Formula.entails s f)
+
+  def Proof.size {s} (f : Formula language) (h : s ⊢ f) : Nat :=
+    let x : Inhabited Nat := 
+    match h with
+    | ax .. => ⟨0⟩
+    | weaken h1 h2 => ⟨h2.size + 1⟩
+    | and_intro h1 h2 => ⟨h1.size + h2.size + 1⟩
+    | and_elim_left h1 => ⟨h1.size + 1⟩
+    | and_elim_right h1 => ⟨h1.size + 1⟩
+    | or_intro_left h1 h2 => ⟨h2.size + 1⟩
+    | or_intro_right h1 h2 => ⟨h2.size + 1⟩
+    | or_elim h1 h2 h3 => ⟨h1.size + h2.size + h3.size + 1⟩
+    | imp_intro h1 => ⟨h1.size + 1⟩
+    | imp_elim h1 h2 => ⟨h1.size + h2.size + 1⟩
+    | bot_elim h1 h2 => ⟨h2.size + 1⟩
+    | lem h1 => ⟨0⟩
+    | all_intro h1 h2 h3 => ⟨h3.size + 1⟩
+    | all_elim h1 h2 => ⟨h2.size + 1⟩
+    | ex_intro h1 => ⟨h1.size + 1⟩
+    | ex_elim h1 h2 h3 h4 => ⟨h3.size + h4.size + 1⟩
+    | eq_intro h1 => ⟨0⟩
+    | eq_elim h1 h2 h3 h4 h5 => ⟨h4.size + h5.size + 1⟩
+  x.1
+
+
+  theorem Formula.isTrueUnder_invariant_of_not_Mem {language} {f} {x : Var}
+    (hx : x ∉ f) (i : Interpretation language) (d : i.domain)
+    : (⊨[i] f) ↔ ⊨[i⟦x := d⟧] f := ⟨by
+      intro h; induction f with
+      | and f g hf hg =>
+          rw [Mem.Mem_and_iff] at hx; exact ⟨hf (λ c => hx (.inl c)) h.1, hg (λ c => hx (.inr c)) h.2⟩
+      | or f g hf hg =>
+          rw [Mem.Mem_or_iff] at hx; match h with
+          | .inl h => exact Or.inl $ hf (λ c => hx (.inl c)) h
+          | .inr h => exact Or.inr $ hg (λ c => hx (.inr c)) h
+      | _ => sorry
+      , sorry⟩
+
+  theorem Proof.soundness {f : Formula language} {s} : (s ⊢ f) → s ⊨ f
+    | ax h1 => λ i hs => hs _ h1
+    | weaken h1 h2 => λ i hs => soundness h2 i λ x hx => hs x (.tail h1 hx)
+    | and_intro h1 h2 => λ i hs => ⟨soundness h1 i hs, soundness h2 i hs⟩
+    | and_elim_left h1 => λ i hs => (soundness h1 i hs).1
+    | and_elim_right h1 => λ i hs => (soundness h1 i hs).2
+    | or_intro_left h1 h2 => λ i hs => Or.inl (soundness h2 i hs)
+    | or_intro_right h1 h2 => λ i hs => Or.inr (soundness h2 i hs)
+    | or_elim h1 h2 h3 => λ i hs => match soundness h1 i hs with
+      | .inl h1 => soundness h2 i hs h1
+      | .inr h1 => soundness h3 i hs h1
+    | imp_intro h1 => λ i hs => 
+      λ b => soundness h1 i λ x => λ | .head _ => b | .tail _ hx => hs _ hx
+    | imp_elim h1 h2 => λ i hs => soundness h2 i hs (soundness h1 i hs)
+    | bot_elim h1 h2 => λ i hs => (soundness h2 i hs).elim
+    | lem h1 => λ i hs => Classical.em _
+    | all_intro x h2 h3 => λ i hs =>
+      λ d => soundness h3 i⟦x := d⟧ λ g hg =>
+        (g.isTrueUnder_invariant_of_not_Mem (h2 g hg) i d).mp (hs g hg)
+    | all_elim (x := x) (t := t) h1 h2 => λ i hs => 
+      let j := i⟦x := ⟦t | i⟧⟧
+      have := soundness h2 j sorry sorry
+      sorry --needs a lemma
+    | ex_intro .. => sorry
+    | ex_elim .. => sorry
+    | eq_intro .. => sorry
+    | eq_elim .. => sorry
+  termination_by _ f h => h.size
+  decreasing_by simp_wf; dsimp [size]; simp_arith
+
+
+  theorem Formula.isTrueUnder_subst_iff {language} {f} {x} {t} (i : Interpretation language) (ht)
+  : (⊨[i] f[x := t, ht]) ↔ ⊨[i⟦x := ⟦t | i⟧⟧] f :=
+    match f, ht with
+    | .and f g, .and h1 h2 => by
+      dsimp [subst, isTrueUnder]
+      rw [isTrueUnder_subst_iff i h1, isTrueUnder_subst_iff i h2]
+    | or f g, .or h1 h2 => by
+      dsimp [subst, isTrueUnder]
+      rw [isTrueUnder_subst_iff i h1, isTrueUnder_subst_iff i h2]
+    | imp f g, .imp h1 h2 => by
+      dsimp [subst, isTrueUnder]
+      rw [isTrueUnder_subst_iff i h1, isTrueUnder_subst_iff i h2]
+    | bot, _ => by
+      simp [subst, isTrueUnder]
+    | propVar p, _ => by
+      simp [subst, isTrueUnder]
+      exact ⟨id, id⟩
+    | app n f l, h1 => by
+      simp [subst]
+      simp [subst, isTrueUnder]
+      -- have := isTrueUnder_subst_iff i h1
+      sorry
+    | all x p, .all _ _ h3 => sorry
+    | ex x p, .ex _ _ h3 => sorry
+    | eq a b, _ => sorry
+
   end
 end
 
